use Data.List.Sigma

Cslib/Computability/LambdaCalculus/LocallyNameless/Stlc/Context.lean
@@ -7,6 +7,7 @@ Authors: Chris Henson
 import Cslib.Computability.LambdaCalculus.LocallyNameless.Untyped.AesopRuleset
 import Mathlib.Data.Finset.Defs
 import Mathlib.Data.Finset.Dedup
+import Mathlib.Data.List.Sigma
 
 /-! # λ-calculus
 
@@ -21,18 +22,16 @@ variable {Var : Type u} {Ty : Type v} [DecidableEq Var]
 namespace LambdaCalculus.LocallyNameless.Stlc
 
 /-- A typing context is a list of free variables and corresponding types. -/
-abbrev Ctx (Var : Type u) (Ty : Type v) := List (Var × Ty)
+abbrev Ctx (Var : Type u) (Ty : Type v) := List ((_ : Var) × Ty)
 
 namespace Ctx
 
 /-- The domain of a context is the finite set of free variables it uses. -/
 @[simp]
-def dom : Ctx Var Ty → Finset Var := List.toFinset ∘ List.map Prod.fst
+def dom : Ctx Var Ty → Finset Var := List.toFinset ∘ List.keys
 
 /-- A well-formed context. -/
-inductive Ok : Ctx Var Ty → Prop
-| nil : Ok []
-| cons : Ok Γ → x ∉ Γ.dom → Ok ((x,σ) :: Γ)
+abbrev Ok : Ctx Var Ty → Prop := List.NodupKeys
 
 variable {Γ Δ : Ctx Var Ty}
 
@@ -41,20 +40,14 @@ theorem dom_perm_mem_iff (h : Γ.Perm Δ) {x : Var} :
     x ∈ Γ.dom ↔ x ∈ Δ.dom := by
   induction h <;> aesop
 
+omit [DecidableEq Var] in
 /-- Context well-formedness is preserved on permuting a context. -/
 @[aesop safe forward (rule_sets := [LambdaCalculus.LocallyNameless.ruleSet])]
-theorem perm (h : Γ.Perm Δ) : Ok Γ → Ok Δ := by
-  induction h <;> intro Γ_ok
-  case cons perm ih =>
-    cases Γ_ok
-    case cons ok_Γ nmem => exact (ih ok_Γ).cons $ (dom_perm_mem_iff perm).not.mp nmem
-  case nil => constructor
-  case trans => simp_all
-  case swap =>
-    cases Γ_ok
-    case cons ok _ =>
-    cases ok
-    case cons ok _ =>
-      constructor
-      constructor
-      all_goals aesop
+theorem perm (h : Γ.Perm Δ) : Ok Γ → Ok Δ := (List.perm_nodupKeys h).mp
+
+omit [DecidableEq Var] in
+@[aesop safe forward (rule_sets := [LambdaCalculus.LocallyNameless.ruleSet])]
+theorem strengthen : (Δ ++ ⟨x, σ⟩ :: Γ).Ok → (Δ ++ Γ).Ok := by
+  intros ok
+  have sl : List.Sublist (Δ ++ Γ) (Δ ++ ⟨x, σ⟩ :: Γ) := by simp
+  exact List.NodupKeys.sublist sl ok
