Cslib/Computability/LambdaCalculus/LocallyNameless/Stlc/Basic.lean
@@ -40,9 +40,9 @@ open Term Ty
 @[aesop unsafe [constructors (rule_sets := [LambdaCalculus.LocallyNameless.ruleSet])]]
 inductive Typing : Ctx Var (Ty Base) → Term Var → Ty Base → Prop
 /-- Free variables, from a context judgement. -/
-| var : Γ.Ok → (x,σ) ∈ Γ → Typing Γ (fvar x) σ
+| var : Γ.Ok → ⟨x,σ⟩ ∈ Γ → Typing Γ (fvar x) σ
 /-- Lambda abstraction. -/
-| abs (L : Finset Var) : (∀ x ∉ L, Typing ((x,σ) :: Γ) (t ^ fvar x) τ) → Typing Γ t.abs (σ ⤳ τ) 
+| abs (L : Finset Var) : (∀ x ∉ L, Typing (⟨x,σ⟩ :: Γ) (t ^ fvar x) τ) → Typing Γ t.abs (σ ⤳ τ) 
 /-- Function application. -/
 | app : Typing Γ t (σ ⤳ τ) → Typing Γ t' σ → Typing Γ (app t t') τ
 
@@ -52,6 +52,7 @@ namespace Typing
 
 variable {Γ Δ Φ : Ctx Var (Ty Base)}
 
+omit [DecidableEq Var] in
 /-- Typing is preserved on permuting a context. -/
 theorem perm : Γ.Perm Δ → Γ ⊢ t ∶ τ → Δ ⊢ t ∶ τ := by 
   intros _ der
@@ -78,9 +79,8 @@ lemma weakening_strengthened :
   case abs σ Γ' τ t xs ext ih =>
     apply Typing.abs (xs ∪ (Γ ++ Φ ++ Δ).dom)
     intros x _
-    have h : (x, σ) :: Γ ++ Δ = (x, σ) :: Γ' := by aesop
-    refine @ih x (by aesop) _ _ Φ h ?_
-    constructor <;> aesop
+    have h : ⟨x, σ⟩ :: Γ ++ Δ = ⟨x, σ⟩ :: Γ' := by aesop
+    refine @ih x ?_ _ _ Φ h ?_ <;> aesop
 
 /-- Weakening of a typing derivation by an additional context. -/
 lemma weakening : Γ ⊢ t ∶ τ → (Γ ++ Δ).Ok → Γ ++ Δ ⊢ t ∶ τ := by
@@ -88,6 +88,7 @@ lemma weakening : Γ ⊢ t ∶ τ → (Γ ++ Δ).Ok → Γ ++ Δ ⊢ t ∶ τ :=
   rw [←List.append_nil (Γ ++ Δ)] at *
   exact weakening_strengthened (by simp_all) ok
 
+omit [DecidableEq Var] in
 /-- Typing derivations exist only for locally closed terms. -/
 lemma lc : Γ ⊢ t ∶ τ → t.LC := by
   intros h
@@ -101,10 +102,10 @@ open Term
 
 /-- Substitution for a context weakened by a single type between appended contexts. -/
 lemma subst_strengthened :
-    (Δ ++ (x, σ) :: Γ) ⊢ t ∶ τ →
+    (Δ ++ ⟨x, σ⟩ :: Γ) ⊢ t ∶ τ →
     Γ ⊢ s ∶ σ → 
     (Δ ++ Γ) ⊢ (t [x := s]) ∶ τ := by
-  generalize  eq : Δ ++ (x, σ) :: Γ = Φ
+  generalize  eq : Δ ++ ⟨x, σ⟩ :: Γ = Φ
   intros h
   revert Γ Δ
   induction h <;> intros Γ Δ eq der
@@ -113,28 +114,39 @@ lemma subst_strengthened :
     simp only [subst_fvar]
     rw [←eq] at mem
     rw [←eq] at ok
-    cases (Ctx.perm (by aesop) ok : @Ctx.Ok Var (Ty Base) _ ((x, σ) :: Δ ++ Γ))
+    cases (Ctx.perm (by aesop) ok : Ctx.Ok (⟨x, σ⟩ :: Δ ++ Γ))
     case cons ok_weak _ =>
     observe perm : (Γ ++ Δ).Perm (Δ ++ Γ)
     by_cases h : x = x' <;> simp only [h]
-    · rw [show τ = σ by aesop]
+    case neg => aesop
+    case pos nmem =>
+      subst h eq
+      have nmem_Γ : ∀ γ, ⟨x, γ⟩ ∉ Γ := by
+        intros γ _
+        exact nmem x (List.mem_keys.mpr ⟨γ, by aesop⟩) rfl
+      have nmem_Δ : ∀ γ, ⟨x, γ⟩ ∉ Δ := by
+        intros γ _
+        exact nmem x (List.mem_keys.mpr ⟨γ, by aesop⟩) rfl
+      have eq' : τ = σ := by
+        simp only [List.mem_append, List.mem_cons, Sigma.mk.injEq, heq_eq_eq] at mem
+        match mem with | _ => aesop
+      rw [eq']
       refine Typing.perm perm (weakening der ?_)
       exact Ctx.perm (id (List.Perm.symm perm)) ok_weak
-    · aesop
   case abs σ Γ' t T2 xs ih' ih =>
     apply Typing.abs (xs ∪ {x} ∪ (Δ ++ Γ).dom)
     intros x _
     rw [
       subst_def, 
       subst_open_var _ _ _ _ _ der.lc,
-      show (x, σ) :: (Δ ++ Γ) = ((x, σ) :: Δ) ++ Γ by aesop
+      show ⟨x, σ⟩ :: (Δ ++ Γ) = (⟨x, σ⟩ :: Δ) ++ Γ by aesop
       ]
     apply ih 
     all_goals aesop  
 
 /-- Substitution for a context weakened by a single type. -/
 lemma typing_subst : 
-    (x, σ) :: Γ ⊢ t ∶ τ  → Γ ⊢ s ∶ σ → Γ ⊢ (t [x := s]) ∶ τ := by
+    ⟨x, σ⟩ :: Γ ⊢ t ∶ τ  → Γ ⊢ s ∶ σ → Γ ⊢ (t [x := s]) ∶ τ := by
   intros weak der
   rw [←List.nil_append Γ]
   exact subst_strengthened weak der
@@ -142,7 +154,7 @@ lemma typing_subst :
 /-- Typing preservation for opening. -/
 @[aesop safe forward (rule_sets := [LambdaCalculus.LocallyNameless.ruleSet])]
 theorem preservation_opening {xs : Finset Var} :
-  (∀ x ∉ xs, (x, σ) :: Γ ⊢ m ^ fvar x ∶ τ) → 
+  (∀ x ∉ xs, ⟨x, σ⟩ :: Γ ⊢ m ^ fvar x ∶ τ) → 
   Γ ⊢ n ∶ σ → Γ ⊢ m ^ n ∶ τ
   := by
   intros mem der
